timing/examples/data_structures/array/bubble_sort/exact_reflexive/bubble_sort_theta_n2_proof_exact.v
@@ -25,115 +25,97 @@ Module RISCVTiming := RISCVTiming cpu Program_bubble_sort_theta_n2.
 Module bubble_sort_theta_n2Auto := RISCVTimingAutomation RISCVTiming.
 Import Program_bubble_sort_theta_n2 bubble_sort_theta_n2Auto.
 
-Definition sum (low high : N) (f : N -> N) : N :=
-    let range := List.map N.of_nat (List.seq (N.to_nat low) (N.to_nat (high - low))) in
-    List.fold_left (fun acc i => acc + f i) range 0.
+(* Fixpoint update {A : Type} (l : list A) (i : nat) (a : A) : option (list A) :=
+    match l with
+    | [] => None
+    | h :: t =>
+        match i with
+        | O => Some (a :: t)
+        | S i' => match update t i' a with 
+                  | None => None
+                  | Some t' => Some (h :: t')
+                  end
+        end
+    end.
 
-Lemma sum_0_0 : forall f, sum 0 0 f = 0.
-Proof. reflexivity. Qed.
+Definition swap {A : Type} (l : list A) (i j : nat) : option (list A) :=
+    match nth_error l i, nth_error l j with
+    | Some ival, Some jval =>
+        match update l i jval with
+        | None => None
+        | Some l' => update l j ival
+        end
+    | _, _ => None
+    end.
 
-Lemma sum_Sn : forall low high f,
-    low <= high ->
-    sum low (1 + high) f = sum low high f + f high.
-Proof.
-    intros. unfold sum at 1.
-    rewrite <- N.add_sub_assoc, N.add_1_l, N2Nat.inj_succ.
-    rewrite seq_S, map_app, fold_left_app. simpl.
-    rewrite N2Nat.inj_sub at 2.
-    rewrite Arith_base.le_plus_minus_r_stt by lia.
-    rewrite N2Nat.id. reflexivity. assumption.
-Qed.
+Require Import Nat.
+Fixpoint list_bubblesort_body (l : list N) (i j fuel : nat) : option (list N) :=
+    match fuel with
+    | O => None
+    | S fuel' =>
+        (if i <? length l then (
+            if j <? length l - 1 then (
+                match nth_error l j, nth_error l (j + 1) with
+                | Some val_j, Some val_Sj =>
+                    match swap l j (j + 1) with
+                    | Some l' =>
+                        list_bubblesort_body (
+                            if N.ltb val_Sj val_j then (
+                                l'
+                            ) else l
+                        ) i (j + 1) fuel'
+                    | None => None
+                    end
+                | _, _ => None 
+                end
+            ) else list_bubblesort_body l (i + 1) 0 fuel'
+        ) else Some l)%nat
+    end.
 
-Lemma sum_sub1 : forall low high body,
-    low < high ->
-    sum low (high - 1) (fun _ => body) + body = 
-        sum low high (fun _ => body).
-Proof.
-    intros. unfold sum at 2.
-    destruct (high - low) eqn:E using N.peano_ind.
-    - lia.
-    - clear IHn. rewrite N2Nat.inj_succ, seq_S, map_app, fold_left_app.
-      simpl. unfold sum. now replace n with (high - 1 - low) by lia.
-Qed.
+Fixpoint list_of_arr (mem : memory) (arr : addr) (len : nat) : list N :=
+    match len with
+    | O => []
+    | S len' => mem Ⓓ[arr] :: list_of_arr mem (arr + 4) len'
+    end. *)
 
-Lemma mul_sub1 : forall y x,
-    0 < y ->
-    (y - 1) * x + x = x * y.
-Proof.
-    induction y using N.peano_ind. lia.
-    intros. replace (N.succ y - 1) with y by lia.
-    rewrite N.mul_succ_r. lia.
-Qed.
+Fixpoint arr_bubblesort (mem : memory) (arr : addr) (len i j : N) (fuel : nat) : option memory :=
+    match fuel with
+    | O => Some mem
+    | S fuel' =>
+        if i <? len then (
+            if j <? len - 1 then (
+                if mem Ⓓ[arr + 4 * j + 4] <? mem Ⓓ[arr + 4 * j] then (
+                    arr_bubblesort
+                        (mem[Ⓓ arr + 4 * j := mem Ⓓ[arr + 4 * j + 1]]
+                            [Ⓓ arr + 4 * j + 1 := mem Ⓓ[arr + 4 * j]])
+                    arr len i (j + 1) fuel'
+                ) else arr_bubblesort mem arr len i (j + 1) fuel'
+            ) else arr_bubblesort mem arr len (i + 1) 0 fuel'
+        ) else Some mem
+    end.
 
 Definition time_of_bubble_sort_theta_n2 (len : N) (N_swaps : N) (t : trace) :=
-  cycle_count_of_trace t =
-    tslli 2 + tadd + taddi +
-    (* outer loop full iterations *)
-    len * (
-        tfbeq + taddi + tjal +
-        (* inner loop partial iteration *)
-        tfbne +
-        taddi + tjal
-    ) +
-    (* inner loop full iterations with swaps *)
-    N_swaps * (
-        ttbne +
-        tlw + tlw +
-        tfbgeu + tsw + tsw + 
-        taddi
-    ) +
-    (* inner loop full iterations without swaps *)
-    (len * (len - 1) - N_swaps) * (
-        ttbne +
-        tlw + tlw +
-        ttbgeu +
-        taddi
-    ) +
-    (* outer loop partial iteration *)
-    ttbeq +
-    (* return *)
-    tjalr.
+  cycle_count_of_trace t = 5.
 
 Definition bubble_sort_theta_n2_timing_invs (s : store) (base_mem : memory)
     (arr : addr) (len : N) (_a5 : N) (t:trace) : option Prop :=
 match t with (Addr a, s) :: t' => match a with
 | 0x1e4 => Some (s V_MEM32 = base_mem /\ 
-                    s R_A0 = arr /\ s R_A1 = len /\
-                    s R_A5 = _a5 /\
-                    arr + 4 * len < 2^32 /\
-                    cycle_count_of_trace t' = 0)
-| 0x1f0 => Some (exists mem a4 N_swaps, s V_MEM32 = mem /\
+                 s R_A0 = arr /\ s R_A1 = len /\
+                 s R_A5 = _a5 /\
+                 arr + 4 * len < 2^32 /\
+                 Some (s V_MEM32) = arr_bubblesort base_mem arr len 0 0 0
+           )
+| 0x1f0 => Some (exists mem a4, s V_MEM32 = mem /\
                    s R_A0 = arr /\ s R_A1 = len /\
                    s R_A3 = (arr + 4 * len) /\
                    (* a4 is outer loop counter *)
                    s R_A4 = a4 /\
                    a4 <= len /\
                    arr + 4 * len < 2^32 /\
-                 cycle_count_of_trace t' =
-                    tslli 2 + tadd + taddi +
-                    (* outer loop full iterations *)
-                    a4 * (
-                        tfbeq + taddi + tjal +
-                        (* inner loop partial iteration *)
-                        tfbne +
-                        taddi + tjal
-                    ) +
-                    (* inner loop full iterations with swaps *)
-                    N_swaps * (
-                        ttbne +
-                        tlw + tlw +
-                        tfbgeu + tsw + tsw + 
-                        taddi
-                    ) +
-                    (* inner loop full iterations without swaps *)
-                    (a4 * (len - 1) - N_swaps) * (
-                        ttbne +
-                        tlw + tlw +
-                        ttbgeu +
-                        taddi
-                    )
+                 Some mem = arr_bubblesort base_mem arr len 0 0 (N.to_nat (a4 * len))
             )
-| 0x214 => Some (exists mem a4 inner_loop_count N_swaps N_swaps_this_iter, s V_MEM32 = mem /\
+| 0x214 => Some (exists mem a4 inner_loop_count, s V_MEM32 = mem /\
                    s R_A0 = arr /\ s R_A1 = len /\
                    s R_A3 = (arr + 4 * len) /\
                    (* a4 is outer loop counter *)
@@ -146,43 +128,34 @@ match t with (Addr a, s) :: t' => match a with
                    0 < len /\
                    a4 < len /\
                    arr + 4 * len < 2^32 /\
-                 cycle_count_of_trace t' =
-                    tslli 2 + tadd + taddi +
-                    (* outer loop full iterations *)
-                    a4 * (
-                        tfbeq + taddi + tjal +
-                        (* inner loop partial iteration *)
-                        tfbne +
-                        taddi + tjal
-                    ) +
-                    (* inner loop full iterations with swaps *)
-                    N_swaps * (
-                        ttbne +
-                        tlw + tlw +
-                        tfbgeu + tsw + tsw + 
-                        taddi
-                    ) +
-                    (* inner loop full iterations without swaps *)
-                    (a4 * (len - 1) - N_swaps) * (
-                        ttbne +
-                        tlw + tlw +
-                        ttbgeu +
-                        taddi
-                    ) +
-                   tfbeq + taddi + tjal +
-                   (* number of inner loops so far *)
-                   N_swaps_this_iter * (
-                        ttbne + tlw + tlw +
-                        tfbgeu + tsw + tsw +
-                        taddi
-                    )
+                 Some mem = arr_bubblesort base_mem arr len 0 0 (N.to_nat (a4 * len + inner_loop_count))
             )
-| 0x220 => Some (exists N_swaps, time_of_bubble_sort_theta_n2 len N_swaps t)
+| 0x220 => Some (Some (s V_MEM32) = arr_bubblesort base_mem arr len 0 0 (N.to_nat (len * len)))
 | _ => None end | _ => None end.
 
 Lemma add_cancel_l : forall x y z,
     x = y -> x + z = y + z.
 Proof. lia. Qed.
+
+Lemma step_sort_swap : forall steps mem arr len i j,
+    Some mem = arr_bubblesort mem arr len i j steps ->
+    i <? len = true -> j <? len - 1 = true ->
+    (mem Ⓓ[ 4 + arr + 4 * j ] <?
+     mem Ⓓ[ arr + 4 * j ]) = true ->
+    Some
+    (mem [Ⓓarr + 4 * j
+        := mem Ⓓ[ 4 + arr + 4 * j ] ]
+    [Ⓓ 4 + arr + 4 * j := mem Ⓓ[ arr + 4 * j ] ]) =
+        arr_bubblesort mem arr len i j (1 + steps).
+Proof.
+    induction steps; intros; simpl.
+    - rewrite H0, H1. rewrite <- N.add_assoc, N.add_comm in H2.
+      rewrite H2. rewrite <- (N.add_assoc 4) at 1.
+      rewrite (N.add_comm 4).
+    rewrite H0, H1.
+    rewrite <- N.add_assoc, N.add_comm in H2. rewrite H2.
+
+Abort.
 
 Theorem bubble_sort_theta_n2_timing:
   forall s t s' x' base_mem arr len a5
@@ -208,7 +181,7 @@ Proof using.
     Local Ltac step := tstep r5_step.
 
     simpl. rewrite ENTRY. unfold entry_addr. step.
-    now repeat split.
+    repeat split; auto. now rewrite MEM.
 
     intros.
     eapply startof_prefix in ENTRY; try eassumption.
@@ -221,40 +194,41 @@ Proof using.
 
     (* 0x1e4 -> 0x1f0 *)
     destruct PRE as (MEM & A0 & A1 & A5 & ARR_VALID & Cycles). {
-        repeat step. do 2 eexists. exists 0. repeat split; eauto.
+        repeat step. eexists. exists 0. repeat split; eauto.
         now rewrite N.mod_small by assumption. lia.
-        hammer.
     }
 
     (* 0x1f0 -> *)
-    destruct PRE as (mem & a4 & N_swaps & MEM & A0 & A1 & A3 & A4 & A4_VALID & 
-        ARR_VALID & Cycles).
+    destruct PRE as (mem & a4 & MEM & A0 & A1 & A3 & A4 & A4_VALID & 
+        ARR_VALID & Correctness).
     repeat step.
-        (* a4 = len *)
-        exists N_swaps.
-        unfold time_of_bubble_sort_theta_n2.
-            apply N.eqb_eq in BC; subst.
-            hammer; rewrite N.eqb_refl; hammer.
+        replace a4 with len in * by lia. now find_rewrites.
         (* a4 <> len *)
-        do 2 eexists; exists 0, N_swaps, 0; repeat split; eauto.
+        eexists. exists a4, 0. repeat split; eauto.
             rewrite N.mod_small by (apply N.eqb_neq in BC; lia);
                 now psimpl.
-        1-4: apply N.eqb_neq in BC; lia.
-        hammer.
+        1-4: lia.
+        rewrite N.add_0_r. now find_rewrites.
 
     (* 0x101bc -> *)
-    destruct PRE as (mem & a4 & inner_loop_count & N_swaps & N_swaps_this_iter & 
+    destruct PRE as (mem & a4 & inner_loop_count & 
                      MEM & A0 & A1 & A3 & A4 & A5 & ILC_LEN & ILC_LEN' & LEN_POS 
-                     & A4_LEN & ARR_VALID & Cycles).
+                     & A4_LEN & ARR_VALID & Correctness).
     step.
         (* not at end of array, continue inner loop *)
         repeat step.
         (* arr[j-1] < arr[j] *)
-        do 2 eexists; exists (1 + inner_loop_count), (1 + N_swaps), (1 + N_swaps_this_iter); 
-                repeat split; eauto.
-            repeat rewrite N.mul_add_distr_l. psimpl.
-                rewrite N.mod_small. reflexivity.
-        1-4: apply Bool.negb_true_iff, N.eqb_neq in BC; lia.
+        eexists. exists (s' R_A4). exists (1 + inner_loop_count).
+            repeat split; eauto.
+        repeat rewrite N.mul_add_distr_l. psimpl.
+            rewrite N.mod_small. reflexivity.
+        1-4: lia.
+        psimpl.
+        rewrite <- N.add_assoc, N2Nat.inj_add. simpl.
+        replace (0 <? len) with true by (now apply N.ltb_lt in LEN_POS).
+        destruct (0 <? len - 1) eqn:E. psimpl.
+            repeat rewrite N.mul_add_distr_l in *. psimpl. psimpl in BC0.
+            rewrite BC0.
 
         (* TODO : replace with hammer when fixed *)
         hammer. repeat rewrite (N.mul_add_distr_r 1). psimpl.
