timing/examples/data_structures/array/bubble_sort/tight_bound/bubble_sort_theta_n2_proof.v
@@ -31,8 +31,8 @@ Module RISCVTiming := RISCVTiming cpu Program_bubble_sort_theta_n2.
 Module bubble_sort_theta_n2Auto := RISCVTimingAutomation RISCVTiming.
 Import Program_bubble_sort_theta_n2 bubble_sort_theta_n2Auto.
 
-Definition time_of_bubble_sort_theta_n2 (mem : addr -> N) 
-        (arr : addr) (len : N) (t : trace) :=
+Definition time_of_bubble_sort_theta_n2
+        (len : N) (t : trace) :=
     (* ----------------------------------------- *)
     (* lower bound, return if len = 0 *)
     tslli 2 + tadd + taddi + ttbeq + tjalr <=
@@ -60,19 +60,19 @@ Definition time_of_bubble_sort_theta_n2 (mem : addr -> N)
     (* return *)
     tjalr.
 
-Definition bubble_sort_theta_n2_timing_invs (s : store) (base_mem : addr -> N)
+Definition bubble_sort_theta_n2_timing_invs (s : store) (base_mem : memory)
     (arr : addr) (len : N) (_a5 : N) (t:trace) : option Prop :=
 match t with (Addr a, s) :: t' => match a with
-| 0x1e4 => Some (s V_MEM32 = Ⓜbase_mem /\ 
-                    s R_A0 = Ⓓarr /\ s R_A1 = Ⓓlen /\
-                    s R_A5 = Ⓓ_a5 /\
+| 0x1e4 => Some (s V_MEM32 = base_mem /\ 
+                    s R_A0 = arr /\ s R_A1 = len /\
+                    s R_A5 = _a5 /\
                     arr + 4 * len < 2^32 /\
                     cycle_count_of_trace t' = 0)
-| 0x1f0 => Some (exists mem a4, s V_MEM32 = Ⓜmem /\
-                   s R_A0 = Ⓓarr /\ s R_A1 = Ⓓlen /\
-                   s R_A3 = Ⓓ(arr + 4 * len) /\
+| 0x1f0 => Some (exists mem a4, s V_MEM32 = mem /\
+                   s R_A0 = arr /\ s R_A1 = len /\
+                   s R_A3 = (arr + 4 * len) /\
                    (* a4 is outer loop counter *)
-                   s R_A4 = Ⓓa4 /\
+                   s R_A4 = a4 /\
                    a4 <= len /\
                    arr + 4 * len < 2^32 /\
                    tslli 2 + tadd + taddi <=
@@ -93,12 +93,12 @@ match t with (Addr a, s) :: t' => match a with
                        taddi + tjal
                    )
             )
-| 0x214 => Some (exists mem a4 inner_loop_count, s V_MEM32 = Ⓜmem /\
-                   s R_A0 = Ⓓarr /\ s R_A1 = Ⓓlen /\
-                   s R_A3 = Ⓓ(arr + 4 * len) /\
+| 0x214 => Some (exists mem a4 inner_loop_count, s V_MEM32 = mem /\
+                   s R_A0 = arr /\ s R_A1 = len /\
+                   s R_A3 = (arr + 4 * len) /\
                    (* a4 is outer loop counter *)
-                   s R_A4 = Ⓓa4 /\
-                   s R_A5 = Ⓓ(arr + 4 * (1 + inner_loop_count)) /\
+                   s R_A4 = a4 /\
+                   s R_A5 = (arr + 4 * (1 + inner_loop_count)) /\
                    1 + inner_loop_count <= len /\
                    (* this is here to handle the inductive case where 
                       inner_loop_count is incremented *)
@@ -131,7 +131,7 @@ match t with (Addr a, s) :: t' => match a with
                         taddi
                     )
             )
-| 0x220 => Some (time_of_bubble_sort_theta_n2 base_mem arr len t)
+| 0x220 => Some (time_of_bubble_sort_theta_n2 len t)
 | _ => None end | _ => None end.
 
 Theorem bubble_sort_theta_n2_timing:
@@ -140,10 +140,10 @@ Theorem bubble_sort_theta_n2_timing:
          (ENTRY: startof t (x',s') = (Addr entry_addr, s))
          (MDL: models rvtypctx s)
          (* bindings *)
-         (MEM: s V_MEM32 = Ⓜbase_mem)
-         (A0: s R_A0 = Ⓓarr)
-         (A2: s R_A1 = Ⓓlen)
-         (A5: s R_A5 = Ⓓa5)
+         (MEM: s V_MEM32 = base_mem)
+         (A0: s R_A0 = arr)
+         (A2: s R_A1 = len)
+         (A5: s R_A5 = a5)
          (* array must fit inside the address space without wrapping *)
          (* this shouldn't be necessary but makes the proof easy *)
          (ARR_VALID: arr + 4 * len < 2^32),
@@ -155,7 +155,7 @@ Theorem bubble_sort_theta_n2_timing:
 Proof using.
     intros.
     apply prove_invs.
-    Local Ltac step := time rv_step.
+    Local Ltac step := tstep r5_step.
 
     simpl. rewrite ENTRY. unfold entry_addr. step.
     now repeat split.
@@ -171,7 +171,7 @@ Proof using.
 
     (* 0x1e4 -> 0x1f0 *)
     destruct PRE as (MEM & A0 & A1 & A5 & ARR_VALID & Cycles). {
-        repeat step. eexists. eexists. repeat split; eauto.
+        repeat step. do 2 eexists. repeat split; eauto.
         now rewrite N.mod_small by assumption. lia.
         (* lower bound *)
         hammer.
@@ -184,18 +184,16 @@ Proof using.
         Cycles_low & Cycles_high).
     repeat step.
         (* a4 = len *)
-        unfold time_of_bubble_sort_theta_n2.
-            apply N.eqb_eq in BC; subst.
-            hammer; rewrite N.eqb_refl; hammer.
+        hammer.
         (* a4 <> len *)
         do 2 eexists; exists 0; repeat split; eauto.
-            rewrite N.mod_small by (apply N.eqb_neq in BC; lia);
-                now psimpl.
-            1-4: apply N.eqb_neq in BC; lia.
-            (* lower bound *)
-            hammer.
-            (* upper bound *)
-            hammer.
+        rewrite N.mod_small by (apply N.eqb_neq in BC; lia);
+            now psimpl.
+        1-4: apply N.eqb_neq in BC; lia.
+        (* lower bound *)
+        hammer.
+        (* upper bound *)
+        hammer.
 
     (* 0x101bc -> *)
     destruct PRE as (mem & a4 & inner_loop_count & MEM & A0 & A1 & A3 & A4
@@ -208,22 +206,21 @@ Proof using.
         do 2 eexists; exists (1 + inner_loop_count); repeat split; eauto.
             repeat rewrite N.mul_add_distr_l. psimpl.
             rewrite N.mod_small. reflexivity.
-            1-3: apply Bool.negb_true_iff, N.eqb_neq in BC; lia.
+            1-4: lia.
         hammer. hammer.
         (* arr[j-1 >= arr[j] *)
         do 2 eexists; exists (1 + inner_loop_count); repeat split; eauto.
             repeat rewrite N.mul_add_distr_l. psimpl.
             rewrite N.mod_small. reflexivity.
-            1-3: apply Bool.negb_true_iff, N.eqb_neq in BC; lia.
+            1-4: apply Bool.negb_true_iff, N.eqb_neq in BC; lia.
         hammer. hammer.
         (* at end of array, exit inner loop -> outer loop invariant *)
         apply Bool.negb_false_iff, N.eqb_eq in BC; subst.
         repeat step.
-        eexists. eexists. repeat split; eauto.
-            rewrite N.mod_small by lia. lia.
+        do 2 eexists. repeat split; eauto.
+            rewrite N.mod_small; lia.
         hammer.
-        replace len with (1 + inner_loop_count) by lia.
-        hammer. rewrite BC, N.eqb_refl.
+        replace (s' R_A1) with (1 + inner_loop_count) by lia.
         rewrite N.mod_small by lia. hammer.
 Qed.
 
